src/VmSemantics.v
@@ -124,12 +124,12 @@ Proof.
     assert (
         StVM.st_trace
           (snd (copland_compile t1 {| st_ev := (splitEv_l s e);
-                                      st_trace := m ++ (k ++ [cvm_split n p]);
+                                      st_trace := m ++ (k ++ [Term_Defs.split n p]);
                                       st_pl := p |})) =
          m ++
          StVM.st_trace
          (snd (copland_compile t1 {| st_ev := (splitEv_l s e);
-                                     st_trace := k ++ [cvm_split n p];
+                                     st_trace := k ++ [Term_Defs.split n p];
                                      st_pl := p |}))).
     {
       rewrite <- app_assoc in *.
@@ -174,43 +174,43 @@ Proof.
     assert (
         StVM.st_trace
           (snd (copland_compile t {| st_ev := (splitEv_l s e);
-                                      st_trace := m ++ (k ++ [cvm_splitp n l p a (get_et (splitEv_r s e))]);
+                                      st_trace := m ++ (k ++ [Term_Defs.split n p] ++ [cvm_thread_start n l p a (get_et (splitEv_r s e))]);
                                       st_pl := p |})) =
          m ++
          StVM.st_trace
          (snd (copland_compile t {| st_ev := (splitEv_l s e);
-                                     st_trace := k ++ [cvm_splitp n l p a (get_et (splitEv_r s e))];
+                                     st_trace := k ++ [Term_Defs.split n p] ++ [cvm_thread_start n l p a (get_et (splitEv_r s e))];
                                      st_pl := p |}))).
     {
-      rewrite <- app_assoc in *.
+      repeat rewrite <- app_assoc in *.
       eapply IHt; eauto.
     }
     subst'.
-    df.
+
     rewrite app_assoc in *.
     subst'.
-    df.  
-    subst.
-    tauto.
-
-    (*
-
+    df.
     assert (
-        StVM.st_trace (snd (copland_compile t2{| st_ev := (splitEv_r s e);
-                                                 st_trace := m ++ st_trace0;
-                                                 st_pl := st_pl0 |})) =
-        m ++ StVM.st_trace (snd (copland_compile t2 {| st_ev := (splitEv_r s e);
-                                                       st_trace := st_trace0;
-                                                       st_pl := st_pl0 |}))
+        ((k ++ [Term_Defs.split n p]) ++
+                                      [cvm_thread_start n l p a (get_et (splitEv_r s e))]) =
+        ( k ++ [Term_Defs.split n p; cvm_thread_start n l p a (get_et (splitEv_r s e))])
       ).
-    eapply IHt2; eauto.
+    {
+      rewrite <- app_assoc.
+      tauto.
+    }
+    rewrite H0 in *; clear H0.
+    rewrite Heqp1 in *; clear Heqp1.
+    df.
+    repeat rewrite <- app_assoc in *.
+    df.
     subst'.
     df.
-    subst. 
-    tauto. 
-     *)
-    
+    subst.
+    rewrite <- app_assoc.
+    tauto.
 Defined.
+
 
 (* Instance of st_trace_cumul' where k=[] *)
 Lemma st_trace_cumul : forall t m e p v,
@@ -732,29 +732,77 @@ Proof.
     eauto. 
 Defined.
 
+(*
 Definition cvm_shuffled_events (e1:list CVM_Event) (e2:list CVM_Event): list CVM_Event.
 Admitted.
+ *)
 
-Inductive cvm_to_lts_trace: list CVM_Event -> list CVM_Event -> Prop :=
-| cvm_shuffle: forall cvm_l1 n n0 loc p t et,
+
+
+(*
+
+Inductive cvm_to_lts_event: Ev -> Ev -> Prop :=
+| cvm_cpy: forall n p,
+    cvm_to_lts_event (copy n p) (copy n p)
+| cvm_umeas: forall n p i args tpl tid,
+    cvm_to_lts_event (umeas n p i args tpl tid)
+                     (umeas n p i args tpl tid)
+| cvm_sign: forall n p et,
+    cvm_to_lts_event (sign n p et)
+                     (sign n p et)
+| cvm_hash: forall n p et,
+    cvm_to_lts_event (hash n p et)
+                     (hash n p et)
+| cvm_req: forall n p q t et,
+    cvm_to_lts_event (req n p q t et)
+                     (req n p q t et)
+| cvm_rpy: forall n p q et,
+    cvm_to_lts_event (rpy n p q et)
+                     (rpy n p q et)
+| cvm_split: forall n p,
+    cvm_to_lts_event (Term_Defs.split n p)
+                     (Term_Defs.split n p)
+| cvm_join: forall n p,
+    cvm_to_lts_event (Term_Defs.join n p)
+                     (Term_Defs.join n p).
+                     
+
+Inductive cvm_to_lts_trace: list Ev -> list Ev -> Prop :=
+(*| cvm_remote: forall a n,
+    cvm_to_lts_trace (remote_events a n) (remote_events a n) *)
+| cvm_shuffle: forall cvm_l1 lts_l1 n n0 loc p t et,
+    cvm_to_lts_trace cvm_l1 lts_l1 ->
     cvm_to_lts_trace
-      ([cvm_splitp n loc p t et] ++ cvm_l1 ++ [cvm_joinp n0 loc p t])
-      ([cvm_split n p] ++ (cvm_shuffled_events cvm_l1 (remote_events t p)) ++ [cvm_join n0 p]).
-
-
-
-    cvm_to_lts_trace l1 cvm_l1 ->
-    cvm_to_lts_trace
+      ([cvm_thread_start n loc p t et] ++
+                                       cvm_l1 ++
+                                       [cvm_thread_end n0 loc p t])
       ([Term_Defs.split n p] ++
-       (shuffled_events l1 (lts_remote_events t p)) ++
-       [Term_Defs.join n0 p])
-      ([cvm_splitp n loc p t et] ++ cvm_l1 ++ [cvm_joinp n0 loc p t])
+                             (shuffled_events lts_l1 (remote_events t p)) ++
+                             [join n0 p])
+| cvm_refl_event: forall cvm_e1 lts_e1,
+    cvm_to_lts_event cvm_e1 lts_e1 ->
+    cvm_to_lts_trace [cvm_e1] [lts_e1]
 
 
+    
+(*
+| cvm_refl: forall ls,
+    (
+    (forall n loc p t et,  ~ (In (cvm_thread_start n  loc  p  t et) ls)) /\
+    (forall n0 loc' p' t', ~ (In (cvm_thread_end   n0 loc' p' t')   ls))
+    ) ->
+    cvm_to_lts_trace ls ls
+*)
+| cvm_move: forall tr_lts tr_cvm rest_lts rest_cvm,
+    cvm_to_lts_trace tr_cvm tr_lts ->
+    cvm_to_lts_trace
+      rest_cvm
+      rest_lts ->
+    cvm_to_lts_trace (tr_cvm ++ rest_cvm) (tr_lts ++ rest_lts).
+Hint Constructors cvm_to_lts_trace : core.
 
 
-
-
+(*
 
 Inductive cvm_to_lts_event: Ev -> CVM_Event -> Prop :=
 | cvmlts_copy: forall n p,
@@ -827,6 +875,576 @@ Inductive cvm_to_lts_trace: list Ev -> list CVM_Event -> Prop :=
       (lts_remote_events a n ++ rest_lts)
       (remote_events a n ++ rest_cvm).
 Hint Constructors cvm_to_lts_trace : core.
+ *)
+
+ *)
+
+Axiom thread_bookend_peel: forall t p et etr n l a n0 tr,
+    lstar (conf (unannoPar t) p et) tr (stop p (aeval (unannoPar t) p et)) ->
+    ([cvm_thread_start n l p a etr] ++ tr ++ [cvm_thread_end (Nat.pred n0) l p a] =
+     (shuffled_events tr (remote_events a p))
+    ).
+
+
+Lemma cvm_refines_lts_event_ordering : forall t cvm_tr bits bits' et et' p p',
+    well_formed_r t ->
+    (*Ev_Shape e et -> *)
+    copland_compile t (mk_st (evc bits et) [] p) = (Some tt, (mk_st (evc bits' et') cvm_tr p')) ->
+    lstar (conf (unannoPar t) p et) cvm_tr (stop p (aeval (unannoPar t) p et)).
+Proof.
+  intros t cvm_tr bits bits' et et' p p' H H'.
+  generalizeEverythingElse t.
+  induction t; intros.
+  - (* aasp case *)
+
+     destruct a;
+      df;
+      econstructor; try (econstructor; reflexivity).
+    
+      
+
+  - (* aatt case *)
+    destruct r.
+    repeat (df; try dohtac; df).
+    
+    assert (lstar (conf a n et) (remote_events a n) (stop n (aeval a n et))).
+    {
+      apply remote_LTS.
+    }
+
+    
+
+    (*
+    pose ev_evshape.
+    pose (e0 e).
+    
+    assert (et_fun e = et).
+    {
+      pose ev_evshape.
+      pose (e0 e).
+      eapply evshape_determ.
+      eassumption.
+      eassumption.
+    }
+    rewrite H1. *)
+    
+
+    eapply lstar_tran.
+    econstructor.
+    simpl.
+    eapply lstar_transitive.
+    eapply lstar_strem.
+    cbn.
+    
+    apply H0.
+    jkjke.
+    ff.
+    assert (et' = (aeval a n et)).
+    {
+      erewrite <- remote_Evidence_Type_Axiom.
+      jkjke.
+    }
+    subst.
+    
+      
+
+    econstructor.
+    apply stattstop.
+    econstructor.
+
+
+
+  -  (* alseq case *)
+    do_wf_pieces.
+    edestruct alseq_decomp; eauto.
+    destruct_conjs.
+    destruct x.
+    econstructor.
+    econstructor.
+    subst.
+    eapply lstar_transitive.
+    eapply lstar_stls.
+    df.
+    eapply IHt1.
+    eassumption.
+    eassumption.
+
+    eapply lstar_silent_tran.
+    apply stlseqstop.
+    df.
+    repeat do_pl_immut.
+    subst.   
+    eapply IHt2. (*with (e:= x). *)
+    eassumption.
+    assert (e0 = Term_Defs.eval (unanno (unannoPar t1)) p et).
+    eapply cvm_refines_lts_evidence; eauto.
+
+    subst.
+    rewrite <- eval_aeval.
+    
+    eassumption.
+
+
+  -    (* abseq case *)
+    do_wf_pieces.
+    destruct r; destruct s; destruct s; destruct s0.
+    +
+      df.
+      vmsts.
+      dosome.
+      df.
+
+      do_suffix blah.
+      do_suffix blah'.
+      destruct_conjs; subst.
+      repeat do_restl.
+      
+      repeat do_pl_immut.
+      subst.
+      repeat rewrite <- app_assoc.
+
+      eapply lstar_tran.
+      econstructor.
+      simpl.
+
+      eapply lstar_transitive.
+      simpl.
+
+      eapply lstar_stbsl.  
+      
+      eapply IHt1.
+      eassumption.
+      (*
+    
+    2: {
+      eassumption.
+      } *)
+      eassumption.
+      
+      unfold run_cvm in *.
+      monad_unfold.
+
+      eapply lstar_silent_tran.
+      apply stbslstop.
+      
+      eapply lstar_transitive.
+      eapply lstar_stbsr.
+      
+      eapply IHt2.
+      eassumption.
+      (*
+    2: {
+      eassumption.
+      } *)
+      eassumption.
+      
+      econstructor.
+
+      eapply stbsrstop.
+      econstructor.
+
+
+    +
+      df.
+      vmsts.
+      dosome.
+      df.
+
+      do_suffix blah.
+      do_suffix blah'.
+      destruct_conjs; subst.
+      repeat do_restl.
+      
+      repeat do_pl_immut.
+      subst.
+      repeat rewrite <- app_assoc.
+
+      eapply lstar_tran.
+      econstructor.
+      simpl.
+
+      eapply lstar_transitive.
+      simpl.
+
+      eapply lstar_stbsl.  
+      
+      eapply IHt1.
+      eassumption.
+      (*
+    
+    2: {
+      eassumption.
+      } *)
+      eassumption.
+      
+      unfold run_cvm in *.
+      monad_unfold.
+
+      eapply lstar_silent_tran.
+      apply stbslstop.
+      
+      eapply lstar_transitive.
+      eapply lstar_stbsr.
+      
+      eapply IHt2.
+      eassumption.
+      (*
+    2: {
+      eassumption.
+      } *)
+      eassumption.
+      
+      econstructor.
+
+      eapply stbsrstop.
+      econstructor.
+ 
+    +
+      
+      df.
+      vmsts.
+      dosome.
+      df.
+
+      do_suffix blah.
+      do_suffix blah'.
+      destruct_conjs; subst.
+      repeat do_restl.
+      
+      repeat do_pl_immut.
+      subst.
+      repeat rewrite <- app_assoc.
+
+      eapply lstar_tran.
+      econstructor.
+      simpl.
+
+      eapply lstar_transitive.
+      simpl.
+
+      eapply lstar_stbsl.  
+      
+      eapply IHt1.
+      eassumption.
+      (*
+    2: {
+      eassumption.
+      } *)
+      eassumption.
+      
+      unfold run_cvm in *.
+      monad_unfold.
+
+      eapply lstar_silent_tran.
+      apply stbslstop.
+      
+      eapply lstar_transitive.
+      eapply lstar_stbsr.
+      
+      eapply IHt2.
+      eassumption.
+      (*
+    2: {
+      eassumption.
+      } *)
+      eassumption.
+      
+      econstructor.
+
+      eapply stbsrstop.
+      econstructor.
+    +
+      df.
+      vmsts.
+      dosome.
+      df.
+
+      do_suffix blah.
+      do_suffix blah'.
+      destruct_conjs; subst.
+      repeat do_restl.
+      
+      repeat do_pl_immut.
+      subst.
+      repeat rewrite <- app_assoc.
+
+      eapply lstar_tran.
+      econstructor.
+      simpl.
+
+      eapply lstar_transitive.
+      simpl.
+
+      eapply lstar_stbsl.  
+      
+      eapply IHt1.
+      eassumption.
+      (*
+    2: {
+      eassumption.
+      } *)
+      eassumption.
+      
+      unfold run_cvm in *.
+      monad_unfold.
+
+      eapply lstar_silent_tran.
+      apply stbslstop.
+      
+      eapply lstar_transitive.
+      eapply lstar_stbsr.
+      
+      eapply IHt2.
+      eassumption.
+      (*
+    2: {
+      eassumption.
+      } *)
+      eassumption.
+      
+      econstructor.
+
+      eapply stbsrstop.
+      econstructor.
+
+
+
+
+
+  - (* abpar case *)
+    do_wf_pieces.
+    destruct r; destruct s; destruct s; destruct s0.
+    +
+      df.
+      vmsts.
+      dosome.
+      df.
+
+      do_suffix blah.
+      (*
+      do_suffix blah'. *)
+      destruct_conjs; subst.
+      repeat do_restl.
+      
+      repeat do_pl_immut.
+      subst.
+      repeat rewrite <- app_assoc.
+
+      assert (lstar (conf (unannoPar t) p et) blah (stop p (aeval (unannoPar t) p et))).
+      eauto.
+
+
+
+      
+
+
+
+      eapply lstar_tran.
+      econstructor.
+      simpl.
+
+      assert (
+          (cvm_thread_start n l p a et
+                            :: blah ++ [cvm_thread_end (Nat.pred n0) l p a; join (Nat.pred n0) p]) =
+          (([cvm_thread_start n l p a et] ++
+                                         blah ++ [cvm_thread_end (Nat.pred n0) l p a]) ++ [join (Nat.pred n0) p])).
+      { rewrite front_app.
+        repeat rewrite <- app_assoc.
+        tauto.
+      }
+      subst'.
+      
+
+
+      erewrite thread_bookend_peel.
+
+      eapply lstar_transitive.
+
+      eapply bpar_shuffle.
+      eassumption.
+
+      eapply lstar_tran.
+      apply stbpstop.
+      econstructor.
+      eassumption.
+
+    +
+      df.
+      vmsts.
+      dosome.
+      df.
+
+      do_suffix blah.
+      (*
+      do_suffix blah'. *)
+      destruct_conjs; subst.
+      repeat do_restl.
+      
+      repeat do_pl_immut.
+      subst.
+      repeat rewrite <- app_assoc.
+
+      assert (lstar (conf (unannoPar t) p et) blah (stop p (aeval (unannoPar t) p et))).
+      eauto.
+
+
+
+      
+
+
+
+      eapply lstar_tran.
+      econstructor.
+      simpl.
+
+      assert (
+          (cvm_thread_start n l p a mt
+                            :: blah ++ [cvm_thread_end (Nat.pred n0) l p a; join (Nat.pred n0) p]) =
+          (([cvm_thread_start n l p a mt] ++
+                                         blah ++ [cvm_thread_end (Nat.pred n0) l p a]) ++ [join (Nat.pred n0) p])).
+      { rewrite front_app.
+        repeat rewrite <- app_assoc.
+        tauto.
+      }
+      subst'.
+      
+
+
+      erewrite thread_bookend_peel.
+
+      eapply lstar_transitive.
+
+      eapply bpar_shuffle.
+      eassumption.
+
+      eapply lstar_tran.
+      apply stbpstop.
+      econstructor.
+      eassumption.
+
+
+
+
+
+          +
+      df.
+      vmsts.
+      dosome.
+      df.
+
+      do_suffix blah.
+      (*
+      do_suffix blah'. *)
+      destruct_conjs; subst.
+      repeat do_restl.
+      
+      repeat do_pl_immut.
+      subst.
+      repeat rewrite <- app_assoc.
+
+      assert (lstar (conf (unannoPar t) p mt) blah (stop p (aeval (unannoPar t) p mt))).
+      eauto.
+
+
+
+      
+
+
+
+      eapply lstar_tran.
+      econstructor.
+      simpl.
+
+      assert (
+          (cvm_thread_start n l p a et
+                            :: blah ++ [cvm_thread_end (Nat.pred n0) l p a; join (Nat.pred n0) p]) =
+          (([cvm_thread_start n l p a et] ++
+                                         blah ++ [cvm_thread_end (Nat.pred n0) l p a]) ++ [join (Nat.pred n0) p])).
+      { rewrite front_app.
+        repeat rewrite <- app_assoc.
+        tauto.
+      }
+      subst'.
+      
+
+
+      erewrite thread_bookend_peel.
+
+      eapply lstar_transitive.
+
+      eapply bpar_shuffle.
+      eassumption.
+
+      eapply lstar_tran.
+      apply stbpstop.
+      econstructor.
+      eassumption.
+
+
+
+
+          +
+      df.
+      vmsts.
+      dosome.
+      df.
+
+      do_suffix blah.
+      (*
+      do_suffix blah'. *)
+      destruct_conjs; subst.
+      repeat do_restl.
+      
+      repeat do_pl_immut.
+      subst.
+      repeat rewrite <- app_assoc.
+
+      assert (lstar (conf (unannoPar t) p mt) blah (stop p (aeval (unannoPar t) p mt))).
+      eauto.
+
+
+
+      
+
+
+
+      eapply lstar_tran.
+      econstructor.
+      simpl.
+
+      assert (
+          (cvm_thread_start n l p a mt
+                            :: blah ++ [cvm_thread_end (Nat.pred n0) l p a; join (Nat.pred n0) p]) =
+          (([cvm_thread_start n l p a mt] ++
+                                         blah ++ [cvm_thread_end (Nat.pred n0) l p a]) ++ [join (Nat.pred n0) p])).
+      { rewrite front_app.
+        repeat rewrite <- app_assoc.
+        tauto.
+      }
+      subst'.
+      
+
+
+      erewrite thread_bookend_peel.
+
+      eapply lstar_transitive.
+
+      eapply bpar_shuffle.
+      eassumption.
+
+      eapply lstar_tran.
+      apply stbpstop.
+      econstructor.
+      eassumption.
+Defined.
+
+
+
+
+
+
+
+(*
 
 Lemma cvm_refines_lts_event_ordering : forall t cvm_tr bits bits' et et' p p',
     well_formed_r t ->
@@ -834,7 +1452,7 @@ Lemma cvm_refines_lts_event_ordering : forall t cvm_tr bits bits' et et' p p',
     copland_compile t (mk_st (evc bits et) [] p) = (Some tt, (mk_st (evc bits' et') cvm_tr p')) ->
     exists tr,
     lstar (conf (unannoPar t) p et) tr (stop p (aeval (unannoPar t) p et)) /\
-    cvm_to_lts_trace tr cvm_tr.
+    cvm_to_lts_trace cvm_tr tr.
 Proof.
   intros t cvm_tr bits bits' et et' p p' H.
   generalizeEverythingElse t.
@@ -844,10 +1462,10 @@ Proof.
       df;
       eexists;
       split;
-      econstructor; try econstructor.
-    
-
-
+      econstructor; try econstructor;
+        try (
+            unfold not; intros;
+            invc H0; try solve_by_inversion).
 
     (*
     +
@@ -897,7 +1515,7 @@ Proof.
     destruct r.
     repeat (df; try dohtac; df).
     
-    assert (lstar (conf a n et) (lts_remote_events a n) (stop n (aeval a n et))).
+    assert (lstar (conf a n et) (remote_events a n) (stop n (aeval a n et))).
     {
       
       apply remote_LTS.
@@ -1072,18 +1690,70 @@ Proof.
      
     econstructor.
     econstructor.
+
+    (*
+    split.
+    +
+      intros.
+      unfold not; intros HH;
+        invc HH; try solve_by_inversion.
+     *)
+    
+
+    (*
+    split; intros;
+      try (
+          unfold not; intros HH;
+          invc HH; try solve_by_inversion).
+     *)
+    
+
+
+    
     econstructor.
 
     econstructor.
+
+    (*
+
+    Axiom not_thread_start_remote: forall n loc p t et a q,
+        ~ In (cvm_thread_start n loc p t et) (remote_events a q).
+
+     Axiom not_thread_end_remote: forall n loc p t a q,
+      ~ In (cvm_thread_end n loc p t) (remote_events a q).
+
+     split; intros;
+       try apply not_thread_start_remote;
+       try apply not_thread_end_remote.
+     *)
+    
+      
+
+
+
+    
     (*
     admit. (*econstructor.*) (* TODO: lemma or extra rule in relation?   Done... *)
      
     
     econstructor. *)
-    rewrite remote_Evidence_Type_Axiom.
-    econstructor.
+
+    admit. (* TODO: axiom or lstar lemma *)
+
     econstructor.
     
+    rewrite remote_Evidence_Type_Axiom.
+    econstructor.
+   
+
+    (*
+    split; intros;
+      try (
+          unfold not; intros HH;
+          invc HH; try solve_by_inversion).
+     *)
+    
+   
 
     
     
@@ -1130,6 +1800,16 @@ Proof.
     
     eassumption.
     +
+      econstructor; eauto.
+
+      (*
+      eauto.
+
+      
+
+
+
+      
       invc H9.
       ++
         simpl.
@@ -1145,6 +1825,8 @@ Proof.
       econstructor.
       eauto.
       eauto.
+       *)
+      
 
 
     (*
@@ -1251,8 +1933,37 @@ Proof.
         
         econstructor.
         econstructor.
+
+        (*
+
+        split; intros;
+          try (
+              unfold not; intros HH;
+              invc HH; try solve_by_inversion).
+         *)
+
+        econstructor.
+        
+        
+
+
+        
         econstructor.
         eauto.
+        econstructor.
+        eauto.
+        econstructor.
+
+        (*
+
+        split; intros;
+          try (
+              unfold not; intros HH;
+              invc HH; try solve_by_inversion).
+         *)
+
+        econstructor.
+        
     +
       
       df.
@@ -1340,11 +2051,52 @@ Proof.
         rewrite H9.
         eauto.
          *)
+
+
+
+
+        econstructor.
+        econstructor.
+
+        (*
+
+        split; intros;
+      try (
+          unfold not; intros HH;
+          invc HH; try solve_by_inversion).
+         *)
+        econstructor.
+        
+
+
+        
+        econstructor.
+        eauto.
+        econstructor.
+        eauto.
+        econstructor.
+
+        (*
+
+        split; intros;
+      try (
+          unfold not; intros HH;
+          invc HH; try solve_by_inversion).
+         *)
+        econstructor.
+
+
+
+
+
+        (*
         
         econstructor.
         econstructor.
         econstructor.
         eauto.
+         *)
+        
     +
       df.
       vmsts.
@@ -1431,11 +2183,46 @@ Proof.
         rewrite H9.
         eauto.
          *)
+
+                econstructor.
+                econstructor.
+
+                (*
+
+        split; intros;
+      try (
+          unfold not; intros HH;
+          invc HH; try solve_by_inversion).
+                 *)
+                econstructor.
         
+
+
+        
+        econstructor.
+        eauto.
+        econstructor.
+        eauto.
+        econstructor.
+
+        (*
+
+        split; intros;
+      try (
+          unfold not; intros HH;
+          invc HH; try solve_by_inversion).
+         *)
+        econstructor.
+
+
+
+        (*
         econstructor.
         econstructor.
         econstructor.
         eauto.
+         *)
+        
     +
       df.
       vmsts.
@@ -1522,11 +2309,44 @@ Proof.
         rewrite H9.
         eauto.
          *)
+
+
+                econstructor.
+        econstructor.
+
+        (*
+        split; intros;
+      try (
+          unfold not; intros HH;
+          invc HH; try solve_by_inversion).
+         *)
+        econstructor.
         
+
+
+        
+        econstructor.
+        eauto.
+        econstructor.
+        eauto.
+        econstructor.
+
+        (*
+        split; intros;
+      try (
+          unfold not; intros HH;
+          invc HH; try solve_by_inversion).
+         *)
+        econstructor.
+
+
+        (*
         econstructor.
         econstructor.
         econstructor.
         eauto.
+         *)
+        
 
         
     
@@ -1720,10 +2540,8 @@ Proof.
       edestruct IHt2; eauto. *)
       destruct_conjs.
 
-      Check lts_remote_events.
 
-
-      exists ([Term_Defs.split n p] ++ (shuffled_events x (lts_remote_events a p)) ++
+      exists ([Term_Defs.split n p] ++ (shuffled_events x (remote_events a p)) ++
                                [Term_Defs.join (Nat.pred n0) p]).
 
       
@@ -1795,304 +2613,459 @@ Proof.
         admit.
         rewrite H5; clear H5. *)
 
-        eapply cvm_shuffle.
-        eassumption.
-    +
-            df.
-      vmsts.
-      dosome.
-      df.
-      simpl.
+          
 
-      do_suffix blah.
-      (* do_suffix blah'. *)
-      destruct_conjs; subst.
-      repeat do_restl.
-      
-      repeat do_pl_immut.
-      subst.
-      repeat rewrite <- app_assoc.
-      edestruct IHt; eauto.
-      (*
-      edestruct IHt2; eauto. *)
-      destruct_conjs.
 
-      Check lts_remote_events.
-
-
-      exists ([Term_Defs.split n p] ++ (shuffled_events x (lts_remote_events a p)) ++
-                               [Term_Defs.join (Nat.pred n0) p]).
-
-      
-      split.
-      ++
-
-      eapply lstar_tran.
-      econstructor.
-      simpl.
-
-      eapply lstar_transitive.
-      simpl.
-
-
-
-      simpl.
-      apply bpar_shuffle.
-      eassumption.
-
-
-
-      (*
-
-      eapply lstar_stbparl.
-      eassumption.
-
-      (*
-      
-      eapply IHt1.
-      eassumption. 
-      (*
-    
-    2: {
-      eassumption.
-      } *)
-      eassumption.
-       *)
-      
-      
-      unfold run_cvm in *.
-      monad_unfold.
-
-      (*
-
-      eapply lstar_silent_tran.
-      apply stbplstop. *)
-      
-      eapply lstar_transitive.
-      eapply lstar_stbparr.
-
-      apply remote_LTS.  *)
-      econstructor.
-      eapply stbpstop.
-      econstructor.
-      ++
-
-        (*
-        simpl.
-
-        assert ( (Term_Defs.split n p :: x ++ lts_remote_events a p ++ [join (Nat.pred n0) p]) =
-                 ([Term_Defs.split n p] ++ x ++ lts_remote_events a p ++ [join (Nat.pred n0) p])).
-        admit.
-        rewrite H5; clear H5.
-
-
-
-        assert ((cvm_splitp n l p a et :: blah ++ [cvm_joinp (Nat.pred n0) l p a]) =
-                ([cvm_splitp n l p a et] ++ blah ++ [cvm_joinp (Nat.pred n0) l p a])).
-        admit.
-        rewrite H5; clear H5. *)
-
-        eapply cvm_shuffle.
-        eassumption.
-    +
-      df.
-      vmsts.
-      dosome.
-      df.
-      simpl.
-
-      do_suffix blah.
-      (* do_suffix blah'. *)
-      destruct_conjs; subst.
-      repeat do_restl.
-      
-      repeat do_pl_immut.
-      subst.
-      repeat rewrite <- app_assoc.
-      edestruct IHt; eauto.
-      (*
-      edestruct IHt2; eauto. *)
-      destruct_conjs.
-
-      Check lts_remote_events.
-
-
-      exists ([Term_Defs.split n p] ++ (shuffled_events x (lts_remote_events a p)) ++
-                               [Term_Defs.join (Nat.pred n0) p]).
-
-      
-      split.
-      ++
-
-      eapply lstar_tran.
-      econstructor.
-      simpl.
-
-      eapply lstar_transitive.
-      simpl.
-
-
-
-      simpl.
-      apply bpar_shuffle.
-      eassumption.
-
-
-
-      (*
-
-      eapply lstar_stbparl.
-      eassumption.
-
-      (*
-      
-      eapply IHt1.
-      eassumption. 
-      (*
-    
-    2: {
-      eassumption.
-      } *)
-      eassumption.
-       *)
-      
-      
-      unfold run_cvm in *.
-      monad_unfold.
-
-      (*
-
-      eapply lstar_silent_tran.
-      apply stbplstop. *)
-      
-      eapply lstar_transitive.
-      eapply lstar_stbparr.
-
-      apply remote_LTS.  *)
-      econstructor.
-      eapply stbpstop.
-      econstructor.
-      ++
-
-        (*
-        simpl.
-
-        assert ( (Term_Defs.split n p :: x ++ lts_remote_events a p ++ [join (Nat.pred n0) p]) =
-                 ([Term_Defs.split n p] ++ x ++ lts_remote_events a p ++ [join (Nat.pred n0) p])).
-        admit.
-        rewrite H5; clear H5.
-
-
-
-        assert ((cvm_splitp n l p a et :: blah ++ [cvm_joinp (Nat.pred n0) l p a]) =
-                ([cvm_splitp n l p a et] ++ blah ++ [cvm_joinp (Nat.pred n0) l p a])).
-        admit.
-        rewrite H5; clear H5. *)
-
-        eapply cvm_shuffle.
-        eassumption.
-    +
-      df.
-      vmsts.
-      dosome.
-      df.
-      simpl.
-
-      do_suffix blah.
-      (* do_suffix blah'. *)
-      destruct_conjs; subst.
-      repeat do_restl.
-      
-      repeat do_pl_immut.
-      subst.
-      repeat rewrite <- app_assoc.
-      edestruct IHt; eauto.
-      (*
-      edestruct IHt2; eauto. *)
-      destruct_conjs.
-
-      Check lts_remote_events.
-
-
-      exists ([Term_Defs.split n p] ++ (shuffled_events x (lts_remote_events a p)) ++
-                               [Term_Defs.join (Nat.pred n0) p]).
-
-      
-      split.
-      ++
-
-      eapply lstar_tran.
-      econstructor.
-      simpl.
-
-      eapply lstar_transitive.
-      simpl.
-
-
-
-      simpl.
-      apply bpar_shuffle.
-      eassumption.
-
-
-
-      (*
-
-      eapply lstar_stbparl.
-      eassumption.
-
-      (*
-      
-      eapply IHt1.
-      eassumption. 
-      (*
-    
-    2: {
-      eassumption.
-      } *)
-      eassumption.
-       *)
-      
-      
-      unfold run_cvm in *.
-      monad_unfold.
-
-      (*
-
-      eapply lstar_silent_tran.
-      apply stbplstop. *)
-      
-      eapply lstar_transitive.
-      eapply lstar_stbparr.
-
-      apply remote_LTS.  *)
-      econstructor.
-      eapply stbpstop.
-      econstructor.
-      ++
-
-        (*
-        simpl.
-
-        assert ( (Term_Defs.split n p :: x ++ lts_remote_events a p ++ [join (Nat.pred n0) p]) =
-                 ([Term_Defs.split n p] ++ x ++ lts_remote_events a p ++ [join (Nat.pred n0) p])).
-        admit.
-        rewrite H5; clear H5.
-
-
-
-        assert ((cvm_splitp n l p a et :: blah ++ [cvm_joinp (Nat.pred n0) l p a]) =
-                ([cvm_splitp n l p a et] ++ blah ++ [cvm_joinp (Nat.pred n0) l p a])).
-        admit.
-        rewrite H5; clear H5. *)
-
-        eapply cvm_shuffle.
-        eassumption.
 
         
 
+        eapply cvm_shuffle.
+        eassumption.
+    +
+      df.
+      vmsts.
+      dosome.
+      df.
+      simpl.
+
+      do_suffix blah.
+      (* do_suffix blah'. *)
+      destruct_conjs; subst.
+      repeat do_restl.
+      
+      repeat do_pl_immut.
+      subst.
+      repeat rewrite <- app_assoc.
+      edestruct IHt; eauto.
+      (*
+      edestruct IHt2; eauto. *)
+      destruct_conjs.
 
 
+      exists ([Term_Defs.split n p] ++ (shuffled_events x (remote_events a p)) ++
+                               [Term_Defs.join (Nat.pred n0) p]).
+
+      
+      split.
+      ++
+
+      eapply lstar_tran.
+      econstructor.
+      simpl.
+
+      eapply lstar_transitive.
+      simpl.
+
+
+
+      simpl.
+      apply bpar_shuffle.
+      eassumption.
+
+
+
+      (*
+
+      eapply lstar_stbparl.
+      eassumption.
+
+      (*
+      
+      eapply IHt1.
+      eassumption. 
+      (*
+    
+    2: {
+      eassumption.
+      } *)
+      eassumption.
+       *)
+      
+      
+      unfold run_cvm in *.
+      monad_unfold.
+
+      (*
+
+      eapply lstar_silent_tran.
+      apply stbplstop. *)
+      
+      eapply lstar_transitive.
+      eapply lstar_stbparr.
+
+      apply remote_LTS.  *)
+      econstructor.
+      eapply stbpstop.
+      econstructor.
+      ++
+
+        (*
+        simpl.
+
+        assert ( (Term_Defs.split n p :: x ++ lts_remote_events a p ++ [join (Nat.pred n0) p]) =
+                 ([Term_Defs.split n p] ++ x ++ lts_remote_events a p ++ [join (Nat.pred n0) p])).
+        admit.
+        rewrite H5; clear H5.
+
+
+
+        assert ((cvm_splitp n l p a et :: blah ++ [cvm_joinp (Nat.pred n0) l p a]) =
+                ([cvm_splitp n l p a et] ++ blah ++ [cvm_joinp (Nat.pred n0) l p a])).
+        admit.
+        rewrite H5; clear H5. *)
+
+        eapply cvm_shuffle.
+        eassumption.
+    +
+      df.
+      vmsts.
+      dosome.
+      df.
+      simpl.
+
+      do_suffix blah.
+      (* do_suffix blah'. *)
+      destruct_conjs; subst.
+      repeat do_restl.
+      
+      repeat do_pl_immut.
+      subst.
+      repeat rewrite <- app_assoc.
+      edestruct IHt; eauto.
+      (*
+      edestruct IHt2; eauto. *)
+      destruct_conjs.
+
+
+      exists ([Term_Defs.split n p] ++ (shuffled_events x (remote_events a p)) ++
+                               [Term_Defs.join (Nat.pred n0) p]).
+
+      
+      split.
+      ++
+
+      eapply lstar_tran.
+      econstructor.
+      simpl.
+
+      eapply lstar_transitive.
+      simpl.
+
+
+
+      simpl.
+      apply bpar_shuffle.
+      eassumption.
+
+
+
+      (*
+
+      eapply lstar_stbparl.
+      eassumption.
+
+      (*
+      
+      eapply IHt1.
+      eassumption. 
+      (*
+    
+    2: {
+      eassumption.
+      } *)
+      eassumption.
+       *)
+      
+      
+      unfold run_cvm in *.
+      monad_unfold.
+
+      (*
+
+      eapply lstar_silent_tran.
+      apply stbplstop. *)
+      
+      eapply lstar_transitive.
+      eapply lstar_stbparr.
+
+      apply remote_LTS.  *)
+      econstructor.
+      eapply stbpstop.
+      econstructor.
+      ++
+
+        (*
+        simpl.
+
+        assert ( (Term_Defs.split n p :: x ++ lts_remote_events a p ++ [join (Nat.pred n0) p]) =
+                 ([Term_Defs.split n p] ++ x ++ lts_remote_events a p ++ [join (Nat.pred n0) p])).
+        admit.
+        rewrite H5; clear H5.
+
+
+
+        assert ((cvm_splitp n l p a et :: blah ++ [cvm_joinp (Nat.pred n0) l p a]) =
+                ([cvm_splitp n l p a et] ++ blah ++ [cvm_joinp (Nat.pred n0) l p a])).
+        admit.
+        rewrite H5; clear H5. *)
+
+        eapply cvm_shuffle.
+        eassumption.
+    +
+      df.
+      vmsts.
+      dosome.
+      df.
+      simpl.
+
+      do_suffix blah.
+      (* do_suffix blah'. *)
+      destruct_conjs; subst.
+      repeat do_restl.
+      
+      repeat do_pl_immut.
+      subst.
+      repeat rewrite <- app_assoc.
+      edestruct IHt; eauto.
+      (*
+      edestruct IHt2; eauto. *)
+      destruct_conjs.
+
+      exists ([Term_Defs.split n p] ++ (shuffled_events x (remote_events a p)) ++
+                               [Term_Defs.join (Nat.pred n0) p]).
+
+      
+      split.
+      ++
+
+      eapply lstar_tran.
+      econstructor.
+      simpl.
+
+      eapply lstar_transitive.
+      simpl.
+
+
+
+      simpl.
+      apply bpar_shuffle.
+      eassumption.
+
+
+
+      (*
+
+      eapply lstar_stbparl.
+      eassumption.
+
+      (*
+      
+      eapply IHt1.
+      eassumption. 
+      (*
+    
+    2: {
+      eassumption.
+      } *)
+      eassumption.
+       *)
+      
+      
+      unfold run_cvm in *.
+      monad_unfold.
+
+      (*
+
+      eapply lstar_silent_tran.
+      apply stbplstop. *)
+      
+      eapply lstar_transitive.
+      eapply lstar_stbparr.
+
+      apply remote_LTS.  *)
+      econstructor.
+      eapply stbpstop.
+      econstructor.
+      ++
+
+        (*
+        simpl.
+
+        assert ( (Term_Defs.split n p :: x ++ lts_remote_events a p ++ [join (Nat.pred n0) p]) =
+                 ([Term_Defs.split n p] ++ x ++ lts_remote_events a p ++ [join (Nat.pred n0) p])).
+        admit.
+        rewrite H5; clear H5.
+
+
+
+        assert ((cvm_splitp n l p a et :: blah ++ [cvm_joinp (Nat.pred n0) l p a]) =
+                ([cvm_splitp n l p a et] ++ blah ++ [cvm_joinp (Nat.pred n0) l p a])).
+        admit.
+        rewrite H5; clear H5. *)
+
+        eapply cvm_shuffle.
+        eassumption.
+
+
+
+        (*
+
+        Unshelve.
+        eauto.
+        eauto.
+        eauto.
+        eauto.
+        eauto.
+        eauto.
+        exact (aasp (0,0) CPY).
+        exact (aasp (0,0) CPY).
+        eauto.
+        eauto.
+        eauto.
+        eauto.
+        eauto.
+        eauto.
+        eauto.
+        exact (aasp (0,0) CPY).
+        exact (aasp (0,0) CPY).
+        eauto.
+        eauto.
+        eauto.
+        eauto.
+        eauto.
+        eauto.
+        eauto.
+        exact (aasp (0,0) CPY).
+        exact (aasp (0,0) CPY).
+        eauto.
+        eauto.
+        eauto.
+        eauto.
+        eauto.
+        eauto.
+        eauto.
+        exact (aasp (0,0) CPY).
+        exact (aasp (0,0) CPY).
+        eauto.
+        eauto.
+        eauto.
+        eauto.
+        eauto.
+        eauto.
+        eauto.
+        exact (aasp (0,0) CPY).
+        exact (aasp (0,0) CPY).
+        eauto.
+        eauto.
+        eauto.
+        eauto.
+        eauto.
+        eauto.
+        eauto.
+        exact (aasp (0,0) CPY).
+        exact (aasp (0,0) CPY).
+        eauto.
+        eauto.
+        eauto.
+        eauto.
+        eauto.
+        eauto.
+        eauto.
+        exact (aasp (0,0) CPY).
+        exact (aasp (0,0) CPY).
+        eauto.
+        eauto.
+        eauto.
+        eauto.
+        eauto.
+        eauto.
+        eauto.
+        exact (aasp (0,0) CPY).
+        exact (aasp (0,0) CPY).
+        eauto.
+        eauto.
+        eauto.
+        eauto.
+        eauto.
+        eauto.
+        eauto.
+        exact (aasp (0,0) CPY).
+        exact (aasp (0,0) CPY).
+        eauto.
+        eauto.
+        eauto.
+        eauto.
+        eauto.
+        eauto.
+        eauto.
+        exact (aasp (0,0) CPY).
+        exact (aasp (0,0) CPY).
+        eauto.
+        eauto.
+        eauto.
+        eauto.
+        eauto.
+        eauto.
+        eauto.
+        exact (aasp (0,0) CPY).
+        exact (aasp (0,0) CPY).
+        eauto.
+        eauto.
+        eauto.
+        eauto.
+        eauto.
+        eauto.
+        eauto.
+        exact (aasp (0,0) CPY).
+        exact (aasp (0,0) CPY).
+        eauto.
+        eauto.
+        eauto.
+        eauto.
+        eauto.
+        eauto.
+        eauto.
+        exact (aasp (0,0) CPY).
+        exact (aasp (0,0) CPY).
+        eauto.
+        eauto.
+        eauto.
+        eauto.
+        eauto.
+        eauto.
+        eauto.
+        exact (aasp (0,0) CPY).
+        exact (aasp (0,0) CPY).
+        eauto.
+        eauto.
+        eauto.
+        eauto.
+        eauto.
+        eauto.
+        eauto.
+        exact (aasp (0,0) CPY).
+        exact (aasp (0,0) CPY).
+        eauto.
+         *)
+        
+Admitted.
+
+
+  *)      
+
+
+
+
+
+
+
+
+
+
+
+
+
+  
 
 
 
@@ -2401,7 +3374,6 @@ Proof.
       econstructor.
 Defined.
  *)
-Admitted.
 
 (*
     exists tr,
@@ -2412,15 +3384,37 @@ Admitted.
 
 Lemma cvm_refines_lts_event_ordering_corrolary : forall t cvm_tr bits (*bits'*) et (*et'*) p (*p'*),
     well_formed_r t ->
-    (*Ev_Shape e et -> *)
-    (*copland_compile t (mk_st (evc bits et) [] p) = (Some tt, (mk_st (evc bits' et') tr p')) -> *)
     st_trace (run_cvm t
                       (mk_st (evc bits et) [] p)) = cvm_tr ->
-    exists tr,
-    lstar (conf (unannoPar t) p et) tr (stop p (aeval (unannoPar t) p et)) /\
-    cvm_to_lts_trace tr cvm_tr.
-    (*lstar (conf t p et) tr (stop p (aeval t p et)). *)
+    lstar (conf (unannoPar t) p et) cvm_tr (stop p (aeval (unannoPar t) p et)).
 Proof.
+  (*
+  intros.
+  destruct (copland_compile t {| st_ev := (evc bits et); st_trace := []; st_pl := p |}) eqn:hi.
+  simpl in *.
+  vmsts.
+  simpl in *.
+  apply cvm_refines_lts_event_ordering with (t:=t) (tr:=tr) (bits:=bits) (et:=et) (bits':=bits') (et':=et') (p:=p) (p':=st_pl); eauto.
+  
+  try dunit.
+  rewrite hi.
+  unfold run_cvm in *.
+  monad_unfold.
+  rewrite hi in *.
+  simpl in *.
+  subst.
+  solve_by_inversion.
+   *)
+  
+
+
+
+
+
+
+
+
+  
   intros.
   destruct (copland_compile t {| st_ev := (evc bits et); st_trace := []; st_pl := p |}) eqn:hi.
   simpl in *.
@@ -2436,9 +3430,27 @@ Proof.
   }
   subst.
   destruct st_ev.
+
+  unfold run_cvm in *.
+  monad_unfold.
+  rewrite hi in *.
+  simpl in *.
+  Check cvm_refines_lts_event_ordering.
+  (*
+cvm_refines_lts_event_ordering
+     : forall (t : AnnoTermPar) (cvm_tr : list Ev) (bits bits' : EvBits)
+         (et et' : Evidence) (p p' : nat),
+       well_formed_r t ->
+       copland_compile t {| st_ev := evc bits et; st_trace := []; st_pl := p |} =
+       (Some tt, {| st_ev := evc bits' et'; st_trace := cvm_tr; st_pl := p' |}) ->
+       exists tr : list Ev,
+         lstar (conf (unannoPar t) p et) tr (stop p (aeval (unannoPar t) p et)) /\
+         cvm_to_lts_trace cvm_tr tr
+   *)
   
   
-  apply cvm_refines_lts_event_ordering with (t:=t) (*(tr:=tr)*) (bits:=bits) (et:=et) (bits':=e) (et':=e0) (p:=p) (p':=st_pl); eauto.
+  eapply cvm_refines_lts_event_ordering with (t:=t) (cvm_tr:=st_trace) (bits:=bits) (et:=et) (bits':=e) (et':=e0) (p:=p) (p':=st_pl); eauto.
+  (*
   
   try dunit.
   rewrite hi.
@@ -2446,7 +3458,7 @@ Proof.
   monad_unfold.
   rewrite hi in *.
   simpl in *.
-  tauto.
+  tauto. *)
 Defined.
 
 Lemma range_par: forall t,
@@ -2469,8 +3481,10 @@ Proof.
     econstructor; eauto.
 Defined.
 
+
+(*
     Lemma cvm_splitp_contra: forall tr_lts n loc p t et,
-      cvm_to_lts_trace tr_lts [cvm_splitp n loc p t et] ->
+      cvm_to_lts_trace [cvm_thread_start n loc p t et] tr_lts  ->
       False.
     Proof.
       intros.
@@ -2562,13 +3576,723 @@ Defined.
         e1_lts = e2_lts.
       Proof.
       Admitted.
+ *)
+
+
+
+(*
+    well_formed_r t ->
+    (*Ev_Shape e et -> *)
+    copland_compile 
+      t
+      (mk_st (evc bits et) [] 0) =
+    (Some tt, (mk_st (evc bits' et') cvm_tr 0)) ->
+    cvm_to_lts_trace cvm_tr tr ->
+ *)
+
+(*
+Axiom remote_events_non_empty: forall a n,
+    remote_events a n <> [].
+ *)
+
+
+
+
+(*
+Lemma cvm_to_lts_nil_l_contra: forall tr_lts,
+  cvm_to_lts_trace [] tr_lts ->
+  False.
+Proof.
+  intros.
+  dependent induction H.
+  (*
+  +
+    edestruct remote_events_non_empty.
+    eauto.
+   *)
+  
+  +
+    ff.
+    simpl.
+    assert (tr_cvm = [] /\ rest_cvm = []).
+    {
+      Search (_ ++ _ = []).
+      eapply app_eq_nil; eauto.
+    }
+    destruct_conjs; subst.
+    eauto.
+Defined.
+
+Lemma cvm_to_lts_nil_r_contra: forall tr_cvm,
+  cvm_to_lts_trace tr_cvm [] ->
+  False.
+Proof.
+  intros.
+  dependent induction H.
+  (*
+  +
+    edestruct remote_events_non_empty.
+    eauto.
+   *)
+  
+  +
+    ff.
+    simpl.
+    assert (tr_lts = [] /\ rest_lts = []).
+    {
+      Search (_ ++ _ = []).
+      eapply app_eq_nil; eauto.
+    }
+    destruct_conjs; subst.
+    eauto.
+Defined.
+    
+(*
+Lemma cvm_to_lts_nil_l: forall tr_lts,
+    cvm_to_lts_trace [] tr_lts ->
+    tr_lts = [].
+Proof.
+  intros.
+  dependent induction H; intros.
+  -
+    ff.
+  -
+    ff.
+    simpl.
+    assert (tr_cvm = [] /\ rest_cvm = []).
+    {
+      Search (_ ++ _ = []).
+      eapply app_eq_nil; eauto.
+    }
+    destruct_conjs; subst.
+    assert (tr_lts = []) by eauto.
+    assert (rest_lts = []) by eauto.
+    subst.
+    tauto.
+Defined.
+*)
+
+
+Lemma copy_determ: forall n p tr,
+    cvm_to_lts_trace [copy n p] tr ->
+    tr = [copy n p].
+Proof.
+  intros.
+  dependent induction H; intros.
+  (*
+  -
+    tauto.
+   *)
+  
+  -
+    solve_by_inversion.
+  -
+     assert (tr_cvm = [copy n p] /\ rest_cvm = [] \/
+            rest_cvm = [copy n p] /\ tr_cvm = []).
+    {
+      edestruct app_eq_unit.
+      eassumption.
+      destruct_conjs; subst.
+      right; eauto.
+      destruct_conjs; subst.
+      left; eauto.
+    }
+    door; subst.
+    exfalso.
+    eapply cvm_to_lts_nil_l_contra; eauto.
+    exfalso.
+    eapply cvm_to_lts_nil_l_contra; eauto.
+Defined.
+
+    
+    
+(*    
+    
+  invc H.
+  -
+    tauto.
+  -
+    invc H1.
+    tauto.
+  -
+    
+    
+    
+  generalizeEverythingElse H.
+  dependent induction H; intros.
+  -
+    ff.
+  -
+    ff.
+    simpl.
+
+    assert (tr_cvm = [copy n p] /\ rest_cvm = [] \/
+            rest_cvm = [copy n p] /\ tr_cvm = []).
+    {
+      edestruct app_eq_unit.
+      eassumption.
+      destruct_conjs; subst.
+      right; eauto.
+      destruct_conjs; subst.
+      left; eauto.
+    }
+    door;
+      subst.
+    +
+      assert (rest_lts = []).
+      {
+        eapply cvm_to_lts_nil_l; eauto.
+      }
+      subst.
+      rewrite app_nil_r.
+      eauto.
+    +
+      assert (tr_lts = []).
+      {
+        eapply cvm_to_lts_nil_l; eauto.
+      }
+      subst.
+      simpl.
+      eauto.
+Defined.
+*)
+
 
 Lemma cvm_to_lts_determ:
-  forall tr tr' cvm_tr,
-    cvm_to_lts_trace tr cvm_tr ->
-    cvm_to_lts_trace tr' cvm_tr ->
+  forall t p p' bits bits' et et' tr tr' cvm_tr,
+    well_formed_r t ->
+    copland_compile 
+      t
+      (mk_st (evc bits et) [] p) =
+    (Some tt, (mk_st (evc bits' et') cvm_tr p')) ->
+    cvm_to_lts_trace cvm_tr tr ->
+    cvm_to_lts_trace cvm_tr tr' ->
     tr = tr'.
 Proof.
+  intros.
+  generalizeEverythingElse t.
+  induction t; intros.
+  -
+    destruct a; ff.
+    +
+
+      (*
+      invc H2.
+      invc H1.
+      congruence.
+      invc H2.
+      congruence.
+      assert (
+          (tr_cvm = [copy n p'] /\ rest_cvm = []) \/
+          (rest_cvm = [copy n p'] /\ tr_cvm = [])
+        ).
+      {
+        admit.
+      }
+      door; subst.
+      ++
+        exfalso.
+        eapply cvm_to_lts_nil_l_contra; eauto.
+      ++
+        exfalso.
+        eapply cvm_to_lts_nil_l_contra; eauto.
+      ++
+        invc H3.
+        invc H1.
+        congruence.
+        invc H2.
+        congruence.
+
+        assert (
+          (tr_cvm = [copy n p'] /\ rest_cvm = []) \/
+          (rest_cvm = [copy n p'] /\ tr_cvm = [])
+        ).
+      {
+        admit.
+      }
+      door; subst.
+      +++
+        exfalso.
+        eapply cvm_to_lts_nil_l_contra; eauto.
+      +++
+        exfalso.
+        eapply cvm_to_lts_nil_l_contra; eauto.
+      ++
+       *)
+      
+        
+
+        
+        
+        
+      
+        
+      
+
+      
+      assert (tr' = [copy n p']).
+      {
+        eapply copy_determ; eauto.
+      }
+      assert (tr = [copy n p']).
+      {
+        eapply copy_determ; eauto.
+      }
+      congruence.
+    +
+      assert (tr' = [umeas n2 p' n l n0 n1]).
+      {
+        admit.
+      }
+      assert (tr = [umeas n2 p' n l n0 n1]).
+      {
+        admit.
+      }
+      congruence.
+    +
+      assert (tr' = [sign n p' et]).
+      {
+        admit.
+      }
+      assert (tr = [sign n p' et]).
+      {
+        admit.
+      }
+      congruence.
+    +
+      assert (tr' = [hash n p' et]).
+      {
+        admit.
+      }
+      assert (tr = [hash n p' et]).
+      {
+        admit.
+      }
+      congruence.
+  -
+    ff.
+
+    assert (tr' =
+            (req n0 p' n (unanno a) et
+          :: remote_events a n ++
+          [rpy (Nat.pred n1) p' n (get_et (toRemote a n (evc bits et)))])).
+    {
+      admit.
+    }
+
+    assert (tr =
+            (req n0 p' n (unanno a) et
+          :: remote_events a n ++
+          [rpy (Nat.pred n1) p' n (get_et (toRemote a n (evc bits et)))])).
+    {
+      admit.
+    }
+    congruence.
+  -
+    ff.
+    ff.
+    simpl.
+    monad_unfold.
+    ff.
+    ff.
+    simpl.
+    vmsts.
+    dunit.
+    do_wf_pieces.
+    do_suffix blah.
+    do_suffix blah'.
+    destruct_conjs.
+    subst.
+    simpl in *.
+
+    do_restl.
+    destruct st_ev.
+
+    assert (exists tr1 tr2,
+               cvm_to_lts_trace blah' tr1 /\
+               cvm_to_lts_trace blah tr2 /\
+               tr = tr1 ++ tr2).
+    {
+      Lemma cvm_to_lts_lseq_decomp: forall t1 t2 r bits et e e0 bits' et' p st_pl p' blah' blah tr,
+        well_formed_r (alseq_par r t1 t2) ->
+        copland_compile t1 {| st_ev := evc bits et; st_trace := []; st_pl := p |} =
+        (Some tt, {| st_ev := evc e e0; st_trace := blah'; st_pl := st_pl |}) ->
+        
+        copland_compile t2 {| st_ev := evc e e0; st_trace := []; st_pl := st_pl |} =
+        (Some tt, {| st_ev := evc bits' et'; st_trace := blah; st_pl := p' |}) ->
+        cvm_to_lts_trace (blah' ++ blah) tr ->
+        (exists tr1 tr2,
+               cvm_to_lts_trace blah' tr1 /\
+               cvm_to_lts_trace blah tr2 /\
+               tr = tr1 ++ tr2).
+      Proof.
+        intros.
+        generalizeEverythingElse H2.
+        dependent induction H2; intros.
+        -
+          ff.
+          simpl.
+
+          (*
+          assert (
+              (In (cvm_thread_start n loc p t et) blah') /\
+              (In (cvm_thread_end n0 loc p t) blah)
+            ).
+          {
+            admit.
+          }
+           *)
+
+          assert (
+              ( exists ls,
+                  blah' = [cvm_thread_start n loc p t et] ++ ls) /\
+              ( exists ls,
+                  blah = [cvm_thread_end n0 loc p t] ++ ls)
+            ).
+          {
+            admit.
+          }
+          destruct_conjs.
+          
+
+          (*
+          exists blah'.
+          exists blah.
+          split. *)
+          
+          admit.
+        -
+          assert (
+              (blah' = [cvm_e1] /\ blah = []) \/
+              (blah = [cvm_e1] /\ blah' = [])
+            ).
+          {
+            admit.
+          }
+          
+          door.
+          +
+            admit. (* trace from t2 cannot be empty *)
+          +
+            admit. (* trace from t1 cannot be empty *)
+        -
+
+          invc H2_.
+          +
+            assert (rest_cvm = blah).
+            {
+              admit.
+            }
+            rewrite <- H3 in *; clear H3.
+
+            assert (([cvm_thread_start n loc p0 t et0] ++ cvm_l1 ++ [cvm_thread_end n0 loc p0 t]) = blah').
+            {
+              admit.
+            }
+            rewrite <- H3 in *; clear H3.
+
+            eexists.
+            eexists.
+            split.
+            econstructor.
+            eassumption.
+            split.
+            eassumption.
+            tauto.
+          +
+            assert (exists ls,
+                       blah' = [cvm_e1] ++ ls /\
+                       rest_cvm = ls ++ blah).
+            {
+              admit.
+            }
+            destruct_conjs.
+            subst.
+
+            edestruct IHcvm_to_lts_trace2.
+            2: { eassumption. }
+            2: { eassumption. }
+            2: { eassumption. }
+            
+            
+            
+            
+            
+            
+            eassumption.
+
+            eexists.
+            eexists.
+            split.
+
+           
+          
+            
+                
+            
+          
+                 
+
+
+          
+          exists blah'.
+          exists blah.
+          split.
+          econstructor.
+          admit.
+          split.
+          econstructor.
+          admit.
+          tauto.
+        -
+          
+
+
+          
+          edestruct IHcvm_to_lts_trace1.
+          Focus 2.
+          eassumption.
+          Focus 2.
+          eassumption.
+          Focus 2.
+          eassumption.
+          admit.
+          destruct_conjs.
+          edestruct IHcvm_to_lts_trace2.
+          Focus 2.
+          eassumption.
+          Focus 2.
+          eassumption.
+          Focus 2.
+          eassumption.
+          admit.
+          destruct_conjs.
+          subst.
+          exists (x0 ++ H2).
+          exists (x1 ++ H6).
+          split.
+
+          
+          eassumption.
+          
+          eassumption.
+          
+          
+
+
+
+          
+      Admitted.
+
+      eapply cvm_to_lts_lseq_decomp; eauto.
+      
+    }
+
+    assert (exists tr1 tr2,
+               cvm_to_lts_trace blah' tr1 /\
+               cvm_to_lts_trace blah tr2 /\
+               tr' = tr1 ++ tr2).
+    {
+      eapply cvm_to_lts_lseq_decomp; eauto.
+    }
+    destruct_conjs.
+    subst.
+    assert (H5 = H6) by eauto.
+    assert (H11 = H7) by eauto.
+    subst.
+    tauto.
+  -
+    
+    {
+      eapply IHt1.
+      eassumption.
+      eassumption.
+    
+    
+
+
+    invc H1.
+    
+    +
+      rewrite <- H5 in *; clear H5.
+      invc H2.
+      ++
+        assert (cvm_l0 = cvm_l1).
+        {
+          admit.
+        }
+        assert (n2 = n0).
+        {
+          admit.
+        }
+        subst.
+        
+        
+      
+    
+    
+    
+    
+    
+      
+      
+      
+      
+      
+      
+      
+      
+      
+
+
+      
+      invc H2; try solve_by_inversion.
+      ++
+        invc H1; try solve_by_inversion.
+
+        assert (tr_cvm = [copy n p'] /\ rest_cvm = [] \/
+                rest_cvm = [copy n p'] /\ tr_cvm = []).
+        {
+          admit.
+        }
+        door; subst.
+        +++
+          
+          assert (rest_lts = []).
+          {
+            admit.
+          }
+          subst.
+          repeat rewrite app_nil_r in *.
+          
+          invc H3; try solve_by_inversion.
+        
+
+      
+  
+
+
+
+
+
+
+
+
+
+
+
+
+
+  
+
+  (*
+  intros.
+  generalizeEverythingElse H.
+  dependent induction H; intros.
+  -
+    invc H0.
+    +
+      assert (cvm_l0 = cvm_l1).
+      {
+        admit.
+      }
+      assert (n2 = n0).
+      {
+        admit.
+      }
+      
+      subst.
+      find_apply_hyp_hyp.
+      subst.
+      tauto.
+    +
+      destruct_conjs.
+      specialize H0 with (n1:=n) (loc0:=loc) (p0:=p) (t0:=t) (et0:=et).
+      unfold not in H0.
+      exfalso.
+      eapply H0.
+      econstructor.
+      tauto.
+    +
+      assert (
+          (tr_cvm =
+           [cvm_thread_start n loc p t et] ++ cvm_l1 ++ [cvm_thread_end n0 loc p t] /\
+           rest_cvm = []) \/
+          (rest_cvm =
+           [cvm_thread_start n loc p t et] ++ cvm_l1 ++ [cvm_thread_end n0 loc p t] /\
+           tr_cvm = [])
+        ). (* TODO: one more "in between" case *)
+      {
+        admit.
+      }
+      door; subst.
+      ++
+        clear H1.
+        assert (rest_lts = []).
+        {
+          admit.
+        }
+        subst.
+        rewrite app_nil_r.
+        clear H3.
+
+
+
+        (*
+        
+        invc H2.
+        +++
+          assert (cvm_l0 = cvm_l1).
+          {
+            admit.
+          }
+          assert (n2 = n0).
+          {
+            admit.
+          }
+          assert (rest_lts = []).
+          {
+            admit.
+          }
+          assert (lts_l1 = lts_l0).
+          {
+            eapply IHcvm_to_lts_trace.
+            subst.
+            eassumption.
+          }
+          
+          subst.
+          rewrite app_nil_r.
+          tauto.
+        +++
+          admit.
+        +++
+          assert (rest_lts = []).
+          {
+            admit.
+          }
+          subst.
+          rewrite app_nil_r.
+          clear H3.
+          
+          
+          
+          
+      
+      
+      
+ *)     
+      
+      
+*)
+
+
+    
+  Admitted.
+
+
+
+  (*
   intros.
   generalizeEverythingElse H.
   dependent induction H; intros.
@@ -2894,33 +4618,51 @@ Proof.
 
     
 Admitted.
+*)   (* END cvm_to_lts_determ attempt *)
 
-Theorem cvm_respects_event_system' : forall t tr cvm_tr ev0 ev1 bits bits' et et',
+*)
+
+Theorem cvm_respects_event_system' : forall t cvm_tr ev0 ev1 bits bits' et et',
     well_formed_r t ->
     (*Ev_Shape e et -> *)
     copland_compile 
       t
       (mk_st (evc bits et) [] 0) =
     (Some tt, (mk_st (evc bits' et') cvm_tr 0)) ->
-    cvm_to_lts_trace tr cvm_tr ->
+    (*cvm_to_lts_trace cvm_tr tr -> *)
     prec (ev_sys (unannoPar t) 0 et) ev0 ev1 ->
-    earlier tr ev0 ev1.
+    earlier cvm_tr ev0 ev1.
 Proof.
   intros.
+  eapply ordered.
+  eapply wfr_implies_wfrannt; eauto.
+  eapply cvm_refines_lts_event_ordering; eauto.
+  eassumption.
+Defined.
+
+(*
+
+
+
+
+  
   edestruct cvm_refines_lts_event_ordering.
   eassumption.
   eassumption.
   destruct_conjs.
+  (*
   assert (x = tr).
   {
     eapply cvm_to_lts_determ; eauto.
-
   }
   subst.
+   *)
+  
   eapply ordered.
   eapply wfr_implies_wfrannt; eauto.
   eassumption.
   eassumption.
+*)
   
 
 
@@ -2978,17 +4720,508 @@ Defined.
   eapply ordered with (p:=0) (e:=et); eauto.
   eapply wfr_implies_wfrannt; eauto.
 Defined.
-*)
+ *)
 
-Theorem cvm_respects_event_system : forall t tr ev0 ev1 bits bits' et et' t',
-    t = annotated t' ->
+Lemma anno_unanno_par: forall a l l' annt,
+    anno_par a l = (l', annt) ->
+    unannoPar annt = a.
+Proof.
+  intros.
+  generalizeEverythingElse a.
+  induction a; intros.
+  -
+    ff.
+  -
+    ff.
+  -
+    ff.
+    assert (unannoPar a = a1) by eauto.
+    assert (unannoPar a0 = a2) by eauto.
+    congruence.
+  -
+    ff.
+    assert (unannoPar a = a1) by eauto.
+    assert (unannoPar a0 = a2) by eauto.
+    congruence.
+  -
+    ff.
+    assert (unannoPar a = a1) by eauto.
+    congruence.
+Defined.
+
+Lemma fst_annopar: forall a a' l l',
+    anno_par a l = (l', a') ->
+    fst (range a) = fst (Term_Defs.range_par a').
+Proof.
+  intros.
+  generalizeEverythingElse a.
+  destruct a; intros; ff.
+Defined.
+
+
+(*
+Lemma snd_annopar: forall a2_1 a2_2 l' l3 a2 l0' a3,
+    anno_par a2_1 l' = (l3, a2) ->
+    anno_par a2_2 l3 = (l0', a3) ->
+    snd (Term_Defs.range_par a2) = fst (Term_Defs.range_par a3).
+Proof.
+  intros.
+  generalizeEverythingElse a2_2.
+  induction a2_2; intros.
+  -
+    ff.
+Admitted.
+ *)
+
+
+Lemma snd_annopar_snd: forall a a' l l',
+    anno_par a l = (l', a') ->
+    Term_Defs.range_par a' = range a.
+Proof.
+  intros.
+  generalizeEverythingElse a.
+  induction a; intros; ff.
+Defined.
+
+Lemma wfr_par_irrel: forall a2 l l' l0 l0' a0 a0',
+    well_formed_r_annt a2 ->
+    anno_par a2 l' = (l0', a0') ->
+    anno_par a2 l = (l0, a0) ->
+    well_formed_r a0 ->
+    well_formed_r a0'.
+Proof.
+  intros.
+  unfold annotated_par in *.
+  (*
+      unfold anno_par in H.
+      repeat break_let.
+      simpl.
+      fold anno_par in *. *)
+  generalizeEverythingElse a2.
+  induction a2; intros.
+  -
+    ff.
+  -
+    ff.
+  -
+    ff.
+    invc H2.
+    invc H.
+    
+    assert (well_formed_r a2).
+    {
+      eauto.
+    }
+    assert (well_formed_r a3).
+    {
+      eauto.
+    }
+
+    (*
+
+        assert (a1 = a3).
+        {
+          eapply anno_par_same; eauto.
+        }
+        assert (a = a2).
+        {
+          eapply anno_par_same; eauto.
+        }
+        subst.
+     *)
+    
+
+    econstructor.
+    eassumption.
+    eassumption.
+    destruct r.
+    simpl in *.
+    subst.
+    erewrite <- fst_annopar.
+    erewrite <- fst_annopar.
+    reflexivity.
+    eassumption.
+    eassumption.
+    erewrite snd_annopar_snd.
+    erewrite snd_annopar_snd.
+    2: { eassumption. }
+    2: { eassumption. }
+    subst'.
+    subst'.
+    congruence.
+
+    (*
+
+    eapply snd_annopar.
+    eassumption.
+    eassumption.
+    subst'. *)
+
+    assert (
+        Term_Defs.range_par a1 =
+        Term_Defs.range_par a3).
+    {
+      rewrite range_par.
+      rewrite range_par.
+      erewrite anno_unanno_par.
+      erewrite anno_unanno_par.
+      reflexivity.
+      eassumption.
+      eassumption.
+    }
+    congruence.
+  -
+    ff.
+    invc H2.
+    invc H.
+    
+    assert (well_formed_r a2).
+    {
+      eauto.
+    }
+    assert (well_formed_r a3).
+    {
+      eauto.
+    }
+
+    (*
+
+        assert (a1 = a3).
+        {
+          eapply anno_par_same; eauto.
+        }
+        assert (a = a2).
+        {
+          eapply anno_par_same; eauto.
+        }
+        subst.
+     *)
+    
+
+    econstructor.
+    eassumption.
+    eassumption.
+    destruct r.
+    simpl in *.
+    subst.
+    subst'.
+    erewrite <- fst_annopar.
+    erewrite <- fst_annopar.
+    reflexivity.
+    eassumption.
+    eassumption.
+
+        erewrite snd_annopar_snd.
+    erewrite snd_annopar_snd.
+    2: { eassumption. }
+    2: { eassumption. }
+    subst'.
+    subst'.
+    congruence.
+
+    (*
+
+    eapply snd_annopar.
+    eassumption.
+    eassumption.
+    subst'. *)
+
+    assert (
+        Term_Defs.range_par a1 =
+        Term_Defs.range_par a3).
+    {
+      rewrite range_par.
+      rewrite range_par.
+      erewrite anno_unanno_par.
+      erewrite anno_unanno_par.
+      reflexivity.
+      eassumption.
+      eassumption.
+    }
+    congruence.
+  -
+    ff.
+    invc H2.
+    
+    invc H.
+    
+    assert (well_formed_r a1).
+    {
+      eauto.
+    }
+    (*
+        assert (well_formed_r a3).
+        {
+          eauto.
+        }
+     *)
+    
+
+    (*
+
+        assert (a1 = a3).
+        {
+          eapply anno_par_same; eauto.
+        }
+        assert (a = a2).
+        {
+          eapply anno_par_same; eauto.
+        }
+        subst.
+     *)
+    
+
+    econstructor.
+    eassumption.
+    eassumption.
+    destruct r.
+    simpl in *.
+    subst.
+    subst'.
+    erewrite <- fst_annopar.
+    erewrite <- fst_annopar.
+    reflexivity.
+    eassumption.
+    eassumption.
+    subst'.
+    subst'.
+    rewrite <- H9.
+
+    (*
+
+        erewrite snd_annopar_snd.
+        2: { eassumption. }
+        
+
+        eapply snd_annopar.
+        eassumption.
+        eassumption.
+        subst'. *)
+
+    assert (
+        Term_Defs.range_par a1 =
+        Term_Defs.range_par a).
+    {
+      rewrite range_par.
+      rewrite range_par.
+      erewrite anno_unanno_par.
+      erewrite anno_unanno_par.
+      reflexivity.
+      eassumption.
+      eassumption.
+    }
+    congruence.
+    congruence.
+Defined.
+
+Lemma wfr_annt_implies_wfr_par: forall a l l' a0,
+    well_formed_r_annt a ->
+    anno_par a l = (l', a0) ->
+    well_formed_r a0.
+Proof.
+
+  
+  intros.
+  generalizeEverythingElse a.
+  induction a; intros;
+    invc H.
+  -
+    try econstructor;
+      ff.
+  -
+    ff.
+  -
+
+
+    (*
+          ff.
+          assert (well_formed_r (annotated_par a1)) by eauto.
+          assert (well_formed_r (annotated_par a2)) by eauto.
+     *)
+    
+
+    
+    unfold anno_par in *.
+    repeat break_let.
+    fold anno_par in *.
+    invc H0.
+    simpl.
+
+    (*
+          assert (a = annotated_par a1).
+          {
+            unfold annotated_par.
+            subst'.
+            tauto.
+          }
+          subst.
+     *)
+    assert (well_formed_r a) by eauto.
+    assert (well_formed_r a3) by eauto.
+    econstructor.
+    eassumption.
+    eassumption.
+    destruct r.
+    simpl in *.
+    subst.
+
+
+
+    eapply fst_annopar; eauto.
+
+        erewrite snd_annopar_snd.
+    erewrite snd_annopar_snd.
+    2: { eassumption. }
+    2: { eassumption. }
+    subst'.
+    congruence.
+
+    
+    
+
+(*
+    eapply snd_annopar; eauto.
+ *)
+    
+
+    subst'.
+
+    rewrite range_par.
+
+    assert (unannoPar a3 = a2).
+    {
+      eapply anno_unanno_par.
+      eassumption.
+    }
+    congruence.
+  -
+    
+
+    (*
+          ff.
+          assert (well_formed_r (annotated_par a1)) by eauto.
+          assert (well_formed_r (annotated_par a2)) by eauto.
+     *)
+    
+
+    
+    unfold anno_par in *.
+    repeat break_let.
+    fold anno_par in *.
+    invc H0.
+    simpl.
+
+    (*
+          assert (a = annotated_par a1).
+          {
+            unfold annotated_par.
+            subst'.
+            tauto.
+          }
+          subst.
+     *)
+    assert (well_formed_r a) by eauto.
+    assert (well_formed_r a3) by eauto.
+    econstructor.
+    eassumption.
+    eassumption.
+    destruct r.
+    simpl in *.
+    subst.
+    rewrite H7.
+
+
+
+    eapply fst_annopar; eauto.
+
+
+
+        erewrite snd_annopar_snd.
+    erewrite snd_annopar_snd.
+    2: { eassumption. }
+    2: { eassumption. }
+    subst'.
+    congruence.
+
+    
+    
+
+(*
+    eapply snd_annopar; eauto.
+ *)
+    
+
+    subst'.
+
+    rewrite range_par.
+
+    assert (unannoPar a3 = a2).
+    {
+      eapply anno_unanno_par.
+      eassumption.
+    }
+    congruence.
+  -
+
+    
+    (*
+          ff.
+          assert (well_formed_r (annotated_par a1)) by eauto.
+          assert (well_formed_r (annotated_par a2)) by eauto.
+     *)
+    
+
+    
+    unfold anno_par in *.
+    repeat break_let.
+    fold anno_par in *.
+    invc H0.
+    simpl.
+
+    (*
+          assert (a = annotated_par a1).
+          {
+            unfold annotated_par.
+            subst'.
+            tauto.
+          }
+          subst.
+     *)
+    assert (well_formed_r a) by eauto.
+    (*
+          assert (well_formed_r a3) by eauto. *)
+    econstructor.
+    eassumption.
+    eassumption.
+    destruct r.
+    simpl in *.
+    subst.
+    rewrite H7.
+
+
+
+    eapply fst_annopar; eauto.
+    rewrite <- H8.
+
+    erewrite snd_annopar_snd; eauto.
+
+    eassumption.
+Defined.
+
+Theorem cvm_respects_event_system : forall t cvm_tr ev0 ev1 bits bits' et et' t',
+    t = annotated_par (annotated t') ->
     (*Ev_Shape e et ->*)
     copland_compile
       t
       (mk_st (evc bits et) [] 0) =
-    (Some tt, (mk_st (evc bits' et') tr 0)) ->
+    (Some tt, (mk_st (evc bits' et') cvm_tr 0)) ->
+     (*cvm_to_lts_trace cvm_tr tr -> *)
+    prec (ev_sys (unannoPar t) 0 et) ev0 ev1 ->
+    earlier cvm_tr ev0 ev1.
+
+            (*
     prec (ev_sys t 0 et) ev0 ev1 ->
-    earlier tr ev0 ev1.
+    earlier tr ev0 ev1. *)
 Proof.
   intros.
   assert (well_formed_r t).
@@ -2997,11 +5230,457 @@ Proof.
     unfold snd in *.
     break_let.
     subst.
-    eapply anno_well_formed_r.
+    assert (well_formed_r_annt (annotated t')).
+    {
+      unfold annotated.
+      unfold snd in *.
+      eapply anno_well_formed_r.
+      rewrite Heqp.
+      reflexivity.
+    }
+    unfold annotated in *.
+    unfold snd in *.
+    rewrite Heqp in *.
+
+    Search "implies".
+
+    Print annotated_par.
+
+    (*
+    Lemma annoPar_range_irrel: forall a2 l l0 a0,
+        anno_par a2 l = (l0, a0) ->
+        range a2 = range (unannoPar a0).
+    Proof.
+    Admitted.
+     *)
+
+    (*
+    Lemma anno_par_same: forall ap l1 l1' l2 l2' annt annt',
+        anno_par ap l1 = (l1', annt) ->
+        anno_par ap l2 = (l2', annt') ->
+        annt = annt'.
+    Proof.
+      intros.
+      generalizeEverythingElse ap.
+      induction ap; intros.
+      -
+        ff.
+      -
+        ff.
+      -
+        ff.
+        assert (a1 = a) by eauto.
+        assert (a2 = a0) by eauto.
+        congruence.
+      -
+        ff.
+        assert (a1 = a) by eauto.
+        assert (a2 = a0) by eauto.
+        congruence.
+      -
+        ff.
+        assert (a0 = a) by eauto.
+        subst.
+        assert (a2 = a0) by eauto.
+        congruence.
+
+    Admitted.
+     *)
+    
+
+
+
+    
+
+
+        
+        
+        
+
+
+(*
+          
+        eapply snd_annopar_snd.
+        erewrite snd_annopar_snd.
+        2: { eassumption. }
+        
+        eassumption.
+
+
+        tauto.
+      - (* abseq case *)
+                ff.
+        invc H2.
+        invc H.
+        
+        assert (well_formed_r a2).
+        {
+          eauto.
+        }
+        assert (well_formed_r a3).
+        {
+          eauto.
+        }
+
+        assert (a1 = a3).
+        {
+          eapply anno_par_same; eauto.
+        }
+        assert (a = a2).
+        {
+          eapply anno_par_same; eauto.
+        }
+        subst.
+
+        econstructor.
+        eassumption.
+        eassumption.
+        destruct r.
+        simpl in *.
+        subst.
+        tauto.
+        eassumption.
+        subst'.
+        tauto.
+      -
+        ff.
+        invc H2.
+        invc H.
+        
+        assert (well_formed_r a1).
+        {
+          eauto.
+        }
+        (*
+        assert (well_formed_r a2_2).
+        {
+          eauto.
+        }
+         *)
+
+        assert (a = a1).
+        {
+          eapply anno_par_same; eauto.
+        }
+        
+
+        (*
+        assert (a1 = a3).
+        {
+          eapply anno_par_same; eauto.
+        }
+        assert (a = a2).
+        {
+          eapply anno_par_same; eauto.
+        }
+         *)
+        
+        subst.
+
+        econstructor.
+        eassumption.
+        eassumption.
+        destruct r.
+        simpl in *.
+        subst.
+        tauto.
+        eassumption.
+        subst'.
+        tauto.
+        Defined.
+ *)
+    
+        
+
+
+    (*
+        Lemma fst_annopar: forall a a' l l',
+          anno_par a l = (l', a') ->
+          fst (range a) = fst (Term_Defs.range_par a').
+        Proof.
+        Admitted.
+
+        eapply fst_annopar; eauto.
+
+        Lemma snd_annopar: forall a2_1 a2_2 l' l3 a2 l0' a3,
+          anno_par a2_1 l' = (l3, a2) ->
+          anno_par a2_2 l3 = (l0', a3) ->
+          snd (Term_Defs.range_par a2) = fst (Term_Defs.range_par a3).
+        
+        
+          simpl.
+          eapply IHa2_2.
+        
+          eapply IHa2_1.
+    
+
+    Lemma wfr_par_irrel: forall a2 l l0 a0,
+        well_formed_r (annotated_par a2) ->
+        anno_par a2 l = (l0, a0) ->
+        well_formed_r a0.
+    Proof.
+      intros.
+      unfold annotated_par in *.
+      (*
+      unfold anno_par in H.
+      repeat break_let.
+      simpl.
+      fold anno_par in *. *)
+      generalizeEverythingElse a2.
+      induction a2; intros.
+      -
+        ff.
+      -
+        ff.
+      -
+        unfold annotated_par in *.
+        unfold anno_par in H.
+        cbn in H0.
+        repeat break_let.
+        fold anno_par in *.
+        simpl in *.
+        ff.
+        invc H.
+        pairs.
+        destruct r.
+        ff.
+        subst.
+        ff.
+        simpl.
+        econstructor.
+        eauto.
+        eauto.
+        simpl.
+        eapply IHa2_2.
+        apply H3
+
+        assert (well_formed_r a).
+        {
+          eapply IHa2_1.
+          subst'.
+          simpl.
+          eassumption.
+          eassumption.
+        }
+
+        assert (well_formed_r a1).
+        {
+          eapply IHa2_2.
+          subst'.
+          simpl.
+          eassumption.
+          eassumption.
+          eapply IHa2_2.
+          subst'.
+          simpl.
+          eassumption.
+        
+          
+
+
+
+
+        
+        repeat break_let.
+        df.
+
+        assert (well_formed_r a2).
+        {
+          eapply IHa2_1.
+          
+
+        
+        invc H.
+        econstructor.
+        eapply IHa2_2.
+        
+        
+        
+
+
+        
+        assert (well_formed_r a2).
+        eapply IHa2_1.
+        
+        find_apply_hyp_hyp.
+        subst'.
+        ff.
+        edestruct IHa2_1.
+        
+        
+
+
+        
+    Admitted.
+     *)
+    
+
+
+
+
+
+
+          
+
+        
+          
+(*
+
+          eapply snd_annopar; eauto.
+
+          subst'.
+
+          rewrite range_par.
+
+          assert (unannoPar a3 = a2).
+          {
+            eapply anno_unanno_par.
+            eassumption.
+          }
+          congruence.
+          
+          
+
+
+
+
+
+
+
+          
+          assert (a0 = annotated_par a2).
+          {
+            unfold annotated_par.
+            subst'.
+          econstructor.
+          eassumption.
+         
+          
+
+
+
+          eapply wfr_par_irrel.
+          2: { eassumption. }
+          eassumption.
+          eassumption.
+
+          eapply wfr_par_irrel.
+          2: { eassumption. }
+          eassumption.
+          eassumption.
+          
+          
+          cbn.
+          Search range.
+          rewrite range_par.
+          rewrite H5.
+
+
+
+          rewrite anno_unanno_par.
+          tauto.
+          repeat rewrite range_par.
+          rewrite anno_unanno_par.
+          rewrite H6.
+
+
+
+          erewrite annoPar_range_irrel; eauto.
+          rewrite H7.
+
+          rewrite range_par.
+
+          erewrite annoPar_range_irrel; eauto.
+        +
+          
+          
+
+
+          
+          rewrite range_par.
+          rewrite H6.
+          rewrite range_par.
+          
+          
+
+
+
+          
+          assert (a0 = annotated_par a2).
+          {
+            unfold annotated_par.
+            subst'.
+            tauto.
+          simpl.
+
+
+          
+          subst.
+          simpl.
+          econstructor.
+          
+          eauto.
+          
+          unfold snd.
+          break_let.
+          repeat break_let.
+          invc Heqp0.
+          econstructor.
+          ff.
+          econstructor.
+          
+
+
+
+        
+        invc H;
+        repeat find_apply_hyp_hyp;
+        repeat rewrite range_par in *;
+        econstructor; eauto.
+       *)
+      
+     
+
+
+
+    unfold annotated_par.
+    assert (exists a', (annotated_par a) = a').
+    {
+      eexists.
+      reflexivity.
+    }
+    destruct_conjs.
+    unfold annotated_par in H3.
+    rewrite H3.
+   
+    
+    eapply wfr_annt_implies_wfr_par with (l:= 0).
     eassumption.
+    assert (anno_par a 0 = (fst (anno_par a 0), snd (anno_par a 0))).
+    {
+      destruct (anno_par a 0); tauto.
+    }
+    rewrite H4.
+    rewrite H3.
+    reflexivity.
   }
+
   eapply ordered with (p:=0) (e:=et); eauto.
+  eapply wfr_implies_wfrannt; eauto.
   eapply cvm_refines_lts_event_ordering; eauto.
+
+  (*
+  eassumption.
+  eassumption.
+  destruct_conjs.
+  assert (tr = x).
+  {
+    eapply cvm_to_lts_determ; eauto.
+  }
+  subst.
+  eassumption.
+   *)
+  
 Defined.
 
 
